nsl/Security.ec
@@ -12,331 +12,59 @@ qed.
 (* ------------------------------------------------------------------------------------------ *)
 
 (* AEAD Reduction *)
-module (Red_AEAD_real (D : A_GWAKE) : A_GAEAD) (O : GAEAD_out) = {
-  module WAKE_O : GWAKE_out = {
-    var b0 : bool
-
-    var state_map: (id * int, role * instance_state) fmap
-  
-    proc init_mem(b: bool) : unit = {
-      b0 <- b;
-      state_map <- empty;
-    }
-  
-    proc gen_pskey = O.gen
-  
-    proc send_msg1(a, i, b) = {
-      var ex, na;
-      var mo <- None;
-  
-      ex <@ O.ex((a, b));
-      if ((a, i) \notin state_map /\ ex) {
-        na <$ dnonce;
-        mo <@ O.enc((a, b), msg1_data a b, na);
-        state_map.[(a, i)] <- (Initiator, IPending (b, witness, na, oget mo) (a, oget mo));
-      }
-      return mo;
-    }
-
-    proc send_msg2(b, j, m1) = {
-      var a, ca, role, st, ex, n, nb;
-      var mo <- None;
-  
-      (a, ca) <- m1;
-      (role, st) <- oget state_map.[(b, j)];
-      ex <@ O.ex((a, b));
-      if ((b, j) \notin state_map /\ ex) {
-        n <@ O.dec((a, b), msg1_data a b, ca);
-        if (n is Some na) {
-          nb <$ dnonce;
-          mo <@ O.enc((a, b), msg2_data a b ca, nb);
-          state_map.[(b, j)] <- (Responder, RPending (a, witness, na, nb, ca, oget mo) m1 (oget mo));
-        } else {
-          state_map.[(b, j)] <- (Responder, Aborted);
-        }
-      }
-      return mo;
-    }
-
-    proc send_msg3(a, i, m2) = {
-      var role, st, b, psk, na, ca, n, skey, ok;
-      var mo <- None;
-  
-      if ((a, i) \in state_map) {
-        (role, st) <- oget state_map.[(a, i)];
-        if (st is IPending s m1) {
-          (b, psk, na, ca) <- s;
-          n <@ O.dec((a, b), msg2_data a b ca, m2);
-          if (n is Some nb) {
-            skey <- prf (na, nb) (a, b);
-            ok <$ dnonce;
-            mo <@ O.enc((a, b), msg3_data a b ca m2, ok);
-            state_map.[(a, i)] <- (Initiator, Accepted ((a, ca), m2, oget mo) skey);
-          } else {
-            state_map.[(a, i)] <- (Initiator, Aborted);
-          }
-        }
-      }
-      return mo;
-    }
-
-    proc send_fin(b, j, m3) = {
-      var role, st, a, psk, na, nb, ca, cb, ok, skey;
-      var mo <- None;
-
-      if ((b, j) \in state_map) {
-        (role, st) <- oget state_map.[(b, j)];
-        if (st is RPending s m1 m2) {
-          (a, psk, na, nb, ca, cb) <- s;
-          ok <@ O.dec((a, b), msg3_data a b ca cb, m3);
-          if (ok is Some nok) {
-            skey <- prf (na, nb) (a, b);
-            state_map.[(b, j)] <- (Responder, Accepted ((a, ca), cb, m3) skey);
-            mo <- Some ();
-          } else {
-            state_map.[(b, j)] <- (Responder, Aborted);
-          }
-        }
-      }
-      return mo;
-    }
-
-    proc rev_skey(a, i) = {
-      var role, st, ps, k;
-      var ko <- None;
-  
-      if ((a, i) \in state_map) {
-        (role, st) <- oget state_map.[(a, i)];
-        match st with
-        | Accepted trace k' => {
-          ps <- get_partners (a, i) (Some trace) role state_map;
-          if (card ps <= 1) {
-            ps <- get_observed_partners (a, i) state_map;
-            if (card ps = 0) {
-              k <- k';
-              ko <- Some k;
-              state_map.[(a, i)] <- (role, Observed trace k);
-            }
-          }
-        }
-        | Observed _ _   => { }
-        | IPending _ _   => { }
-        | RPending _ _ _ => { }
-        | Aborted        => { }
-        end;
-      }
-      return ko;
-    }
-  
-    proc test(a, i) = {
-      var role, st, ps, k;
-      var ko <- None;
- 
-      if ((a, i) \in state_map) {
-        (role, st) <- oget state_map.[(a, i)];
-        match st with
-        | Accepted trace k' => {
-          ps <- get_partners (a, i) (Some trace) role state_map;
-          if (card ps <= 1) {
-            ps <- get_observed_partners (a, i) state_map;
-            if (card ps = 0) {
-              if (b0 = false) {
-                k <- k';
-              } else {
-                k <$ dskey;
-              }
-              ko <- Some k;
-              state_map.[(a, i)] <- (role, Observed trace k);
-            }
-          }
-        }
-        | Observed _ _   => { }
-        | IPending _ _   => { }
-        | RPending _ _ _ => { }
-        | Aborted        => { }
-        end;
-      }
-      return ko;
-    }
+module (Red_AEAD (D : A_GWAKE) : A_GAEAD) (O : GAEAD_out) = {
+  module WAKE_O : GWAKE_out = Game1 with {
+    - var psk_map
+    proc init_mem [ -1 - ]
+    proc gen_pskey [ ^if ~ { O.gen(a, b); } ]
+    proc send_msg1 [
+      var ex : bool
+      ^if + ^ { ex <@ O.ex(a, b); }    
+      ^if ~ ((a, i) \notin state_map /\ ex)
+      [^if.^ca<$ - ^mo<-] ~ { mo <@ O.enc((a, b), msg1_data a b, na); }
+    ]
+    proc send_msg2 [
+      var ex : bool
+      var n : nonce option
+      ^if + ^ { ex <@ O.ex(a, b); }    
+      ^if ~ ((b, j) \notin state_map /\ ex)
+      ^if.^match + ^ { n <@ O.dec((a, b), msg1_data a b, ca); }
+      ^if.^match ~ (n)
+      [^if.^match#Some.^cb<$ - ^mo<-] ~ { mo <@ O.enc((a, b), msg2_data a b ca, nb); }
+    ]
+    proc send_msg3 [
+      var n : nonce option
+      ^if.^match#IPending.^match + ^ { n <@ O.dec((a, b), msg2_data a b ca, m2); }
+      ^if.^match#IPending.^match ~ (n)
+      [^if.^match#IPending.^match#Some.^caf<$ - ^mo<-] ~ { mo <@ O.enc((a, b), msg3_data a b ca m2, ok); }
+    ]
+    proc send_fin [
+      var n : nonce option
+      ^if.^match#RPending.^match + ^ { n <@ O.dec((a, b), msg3_data a b ca cb, m3); }
+      ^if.^match#RPending.^match ~ (n)
+    ]
   }
   
-  proc run() = {
+  proc run(b) = {
     var b';
-    WAKE_O.init_mem(false);
+    WAKE_O.init_mem(b);
     b' <@ D(WAKE_O).run();
     return b';
   }
 }.
-
-module (Red_AEAD_ideal (D : A_GWAKE) : A_GAEAD) (O : GAEAD_out) = {
-  module WAKE_O : GWAKE_out = {
-    var b0 : bool
-
-    var state_map: (id * int, role * instance_state) fmap
-  
-    proc init_mem(b: bool) : unit = {
-      b0 <- b;
-      state_map <- empty;
-    }
-  
-    proc gen_pskey = O.gen
-  
-    proc send_msg1(a, i, b) = {
-      var ex, na;
-      var mo <- None;
-  
-      ex <@ O.ex((a, b));
-      if ((a, i) \notin state_map /\ ex) {
-        na <$ dnonce;
-        mo <@ O.enc((a, b), msg1_data a b, na);
-        state_map.[(a, i)] <- (Initiator, IPending (b, witness, na, oget mo) (a, oget mo));
-      }
-      return mo;
-    }
-
-    proc send_msg2(b, j, m1) = {
-      var a, ca, role, st, ex, n, nb;
-      var mo <- None;
-  
-      (a, ca) <- m1;
-      (role, st) <- oget state_map.[(b, j)];
-      ex <@ O.ex((a, b));
-      if ((b, j) \notin state_map /\ ex) {
-        n <@ O.dec((a, b), msg1_data a b, ca);
-        if (n is Some na) {
-          nb <$ dnonce;
-          mo <@ O.enc((a, b), msg2_data a b ca, nb);
-          state_map.[(b, j)] <- (Responder, RPending (a, witness, na, nb, ca, oget mo) m1 (oget mo));
-        } else {
-          state_map.[(b, j)] <- (Responder, Aborted);
-        }
-      }
-      return mo;
-    }
-
-    proc send_msg3(a, i, m2) = {
-      var role, st, b, psk, na, ca, n, skey, ok;
-      var mo <- None;
-  
-      if ((a, i) \in state_map) {
-        (role, st) <- oget state_map.[(a, i)];
-        if (st is IPending s m1) {
-          (b, psk, na, ca) <- s;
-          n <@ O.dec((a, b), msg2_data a b ca, m2);
-          if (n is Some nb) {
-            skey <- prf (na, nb) (a, b);
-            ok <$ dnonce;
-            mo <@ O.enc((a, b), msg3_data a b ca m2, ok);
-            state_map.[(a, i)] <- (Initiator, Accepted ((a, ca), m2, oget mo) skey);
-          } else {
-            state_map.[(a, i)] <- (Initiator, Aborted);
-          }
-        }
-      }
-      return mo;
-    }
-
-    proc send_fin(b, j, m3) = {
-      var role, st, a, psk, na, nb, ca, cb, ok, skey;
-      var mo <- None;
-
-      if ((b, j) \in state_map) {
-        (role, st) <- oget state_map.[(b, j)];
-        if (st is RPending s m1 m2) {
-          (a, psk, na, nb, ca, cb) <- s;
-          ok <@ O.dec((a, b), msg3_data a b ca cb, m3);
-          if (ok is Some nok) {
-            skey <- prf (na, nb) (a, b);
-            state_map.[(b, j)] <- (Responder, Accepted ((a, ca), cb, m3) skey);
-            mo <- Some ();
-          } else {
-            state_map.[(b, j)] <- (Responder, Aborted);
-          }
-        }
-      }
-      return mo;
-    }
-
-    proc rev_skey(a, i) = {
-      var role, st, ps, k;
-      var ko <- None;
-  
-      if ((a, i) \in state_map) {
-        (role, st) <- oget state_map.[(a, i)];
-        match st with
-        | Accepted trace k' => {
-          ps <- get_partners (a, i) (Some trace) role state_map;
-          if (card ps <= 1) {
-            ps <- get_observed_partners (a, i) state_map;
-            if (card ps = 0) {
-              k <- k';
-              ko <- Some k;
-              state_map.[(a, i)] <- (role, Observed trace k);
-            }
-          }
-        }
-        | Observed _ _   => { }
-        | IPending _ _   => { }
-        | RPending _ _ _ => { }
-        | Aborted        => { }
-        end;
-      }
-      return ko;
-    }
-  
-    proc test(a, i) = {
-      var role, st, ps, k;
-      var ko <- None;
- 
-      if ((a, i) \in state_map) {
-        (role, st) <- oget state_map.[(a, i)];
-        match st with
-        | Accepted trace k' => {
-          ps <- get_partners (a, i) (Some trace) role state_map;
-          if (card ps <= 1) {
-            ps <- get_observed_partners (a, i) state_map;
-            if (card ps = 0) {
-              if (b0 = false) {
-                k <- k';
-              } else {
-                k <$ dskey;
-              }
-              ko <- Some k;
-              state_map.[(a, i)] <- (role, Observed trace k);
-            }
-          }
-        }
-        | Observed _ _   => { }
-        | IPending _ _   => { }
-        | RPending _ _ _ => { }
-        | Aborted        => { }
-        end;
-      }
-      return ko;
-    }
-  }
-  
-  proc run() = {
-    var b';
-    WAKE_O.init_mem(true);
-    b' <@ D(WAKE_O).run();
-    return b';
-  }
-}.
-
 
 (* ------------------------------------------------------------------------------------------ *)
 (* ROM Reduction *)
 
-clone import PROM.FullRO as NROc with
+clone PROM.FullRO as NROc with
   type in_t    <= msg_data * ctxt,
   type out_t   <= nonce,
   op   dout  _ <= dnonce,
-  type d_in_t  <= unit,
+  type d_in_t  <= bool,
   type d_out_t <= bool
 proof *.
 
-module (Red_ROM_real (D : A_GWAKE) : RO_Distinguisher) (O : RO) = {
+module (Red_ROM (D : A_GWAKE) : NROc.RO_Distinguisher) (O : NROc.RO) = {
   module WAKE_O : GWAKE_out = Game4 with {
     proc send_msg1 [
       ^if.^if.^na<$ ~ {na <- witness; O.sample((msg1_data a b, ca)); }
@@ -367,436 +95,41 @@ module (Red_ROM_real (D : A_GWAKE) : RO_Distinguisher) (O : RO) = {
     ]
   }
 
-  proc distinguish() = {
+  proc distinguish(b) = {
     var b';
-    WAKE_O.init_mem(false);
+    WAKE_O.init_mem(b);
     b' <@ D(WAKE_O).run();
     return b';
   }
 }.
-
-module (Red_ROM_ideal (D : A_GWAKE) : RO_Distinguisher) (O : RO) = {
-  module WAKE_O : GWAKE_out = Game4 with {
-    proc send_msg1 [
-      ^if.^if.^na<$ ~ {na <- witness; O.sample((msg1_data a b, ca)); }
-    ]
-
-    proc send_msg2 [
-      ^if.^match#Some.^if.^nb<$ ~ {nb <- witness; O.sample((msg2_data a b ca, cb)); }
-    ]
-
-    proc send_msg3 [
-      ^if.^match#IPending.^match#Some.^if.^ok<$ ~ {
-        ok <- witness;
-        O.sample((msg3_data a b ca m2, caf));
-      }
-      ^if.^match#IPending.^match#Some.^if.^skey<- ~ {
-        na <@ O.get((msg1_data a b, ca));
-        ok <@ O.get((msg2_data a b ca, m2));
-        skey <- prf (na, ok) (a, b);
-      }
-    ]
-
-    proc send_fin [
-      ^if.^match#RPending.^match#Some.^skey<- ~ {
-        na <@ O.get((msg1_data a b, ca));
-        nb <@ O.get((msg2_data a b ca, cb));
-        skey <- prf (na, nb) (a, b);
-      }
-    ]
-  }
-
-  proc distinguish() = {
-    var b';
-    WAKE_O.init_mem(true);
-    b' <@ D(WAKE_O).run();
-    return b';
-  }
-}.
-
 (* ------------------------------------------------------------------------------------------ *)
 (* PRF Reduction *)
-module (Red_PRF_real (D : A_GWAKE) : A_GPRF) (O : GPRF_out) = {
-  module WAKE_O : GWAKE_out = {
-    var b0 : bool
 
-    var dec_map : ((id * id) * msg_data * ctxt, nonce) fmap
-    var bad : bool
-    var state_map : (id * int, role * instance_state) fmap
-    var psk_map : (id * id, pskey) fmap
-  
-    proc init_mem(b: bool) = {
-      b0 <- b;
-      state_map <- empty;
-      psk_map <- empty;
-      bad <- false;
-      dec_map <- empty;
-    }
-  
-    proc gen_pskey(a, b) = {
-      var k;
-  
-      if ((a, b) \notin psk_map) {
-        k <$ dpskey;
-        psk_map.[a, b] <- k;
+module (Red_PRF (D : A_GWAKE) : A_GPRF) (O : GPRF_out) = {
+  module WAKE_O : GWAKE_out = Game5 with {
+    - var prfkey_map
+    proc init_mem [-1 -]
+    proc send_msg3 [
+      var skeyo : skey option
+      [^if.^match#IPending.^match#Some.^if.^ <$ - ^skey<-] ~ {
+        O.gen((msg3_data a b ca m2, caf));
+        skeyo <@ O.f((msg3_data a b ca m2, caf), (a, b));
+        skey <- oget skeyo;
       }
-    }
-  
-    proc send_msg1(a, i, b) = {
-      var ca, mo;
-      
-      mo <- None;
-      if (((a, i) \notin state_map) /\ ((a, b) \in psk_map)) {
-        ca <$ dctxt;
-        bad <- bad \/ exists pk ad, (pk, ad, ca) \in dec_map;
-        if (!bad) {
-          dec_map.[(a, b), msg1_data a b, ca] <- witness;
-          mo <- Some ca;
-          state_map.[a, i] <- (Initiator, IPending (b, witness, witness, ca) (a, ca));
-        }
-      }
-      
-      return mo;
-    }
+    ]
 
-    proc send_msg2(b : id, j : int, m1 : id * ctxt) : ctxt option = {
-      var a, ca, role, st, cb, mo;
-      
-      mo <- None;
-      (a, ca) <- m1;
-      (role, st) <- oget state_map.[b, j];
-      if (((b, j) \notin state_map) /\ ((a, b) \in psk_map)) {
-        if (dec_map.[(a, b), msg1_data a b, ca] is Some na) {
-          cb <$ dctxt;
-          bad <- bad \/ exists pk ad, (pk, ad, cb) \in dec_map;
-          if (!bad) {
-            dec_map.[(a, b), msg2_data a b ca, cb] <- witness;
-            mo <- Some cb;
-            state_map.[b, j] <- (Responder, RPending (a, witness, witness, witness, ca, cb) m1 cb);
-          }
-        } else {
-          state_map.[b, j] <- (Responder, Aborted);
-        }
+    proc send_fin [
+      var skeyo : skey option
+      ^if.^match#RPending.^match#Some.^skey<- ~ {
+        skeyo <@ O.f((msg3_data a b ca cb, m3), (a, b));
+        skey <- oget skeyo;
       }
-      
-      return mo;
-    }
-    
-    proc send_msg3(a : id, i : int, m2 : ctxt) : ctxt option = {
-      var role, st, b, psk, na, ca, skey, caf, mo; 
-      
-      mo <- None;
-      if ((a, i) \in state_map) {
-        (role, st) <- oget state_map.[a, i];
-        match (st) with
-        | IPending s m1 => {
-          (b, psk, na, ca) <- s;
-          if (dec_map.[(a, b), msg2_data a b ca, m2] is Some nb) {
-            caf <$ dctxt;
-            bad <- bad \/ exists pk ad, (pk, ad, caf) \in dec_map;
-            if (!bad) {
-              dec_map.[(a, b), msg3_data a b ca m2, caf] <- witness;
-              mo <- Some caf;
-              O.gen((msg3_data a b ca m2, caf));
-              skey <@ O.f((msg3_data a b ca m2, caf), (a, b));
-              state_map.[a, i] <- (Initiator, Accepted ((a, ca), m2, caf) (oget skey));
-            }
-          } else {
-            state_map.[a, i] <- (Initiator, Aborted);
-          }
-        }
-        | RPending _ _ _ => {}
-        | Accepted _ _ => {}
-        | Observed _ _ => {}
-        | Aborted => {}
-        end;
-      }
-      
-      return mo;
-    }
-
-    proc send_fin(b : id, j : int, m3 : ctxt) : unit option = {
-      var role, st, a, psk, na, nb, ca, cb, skey, mo;
-      
-      mo <- None;
-      if ((b, j) \in state_map) {
-        (role, st) <- oget state_map.[b, j];
-        match (st) with
-        | IPending _ _ => {}
-        | RPending s m1 m2 => {
-          (a, psk, na, nb, ca, cb) <- s;
-          if(dec_map.[(a, b), msg3_data a b ca cb, m3] is Some nok) {
-            skey <@ O.f((msg3_data a b ca cb, m3), (a, b));
-            state_map.[b, j] <- (Responder, Accepted ((a, ca), cb, m3) (oget skey));
-            mo <- Some tt;
-          } else {
-           state_map.[b, j] <- (Responder, Aborted);
-          }
-        }
-        | Accepted _ _ => {}
-        | Observed _ _ => {}
-        | Aborted => {}
-        end;
-      }
-      
-      return mo;
-    }
-
-    proc rev_skey(a, i) = {
-      var role, st, ps, k;
-      var ko <- None;
-  
-      if ((a, i) \in state_map) {
-        (role, st) <- oget state_map.[(a, i)];
-        match st with
-        | Accepted trace k' => {
-          ps <- get_partners (a, i) (Some trace) role state_map;
-          if (card ps <= 1) {
-            ps <- get_observed_partners (a, i) state_map;
-            if (card ps = 0) {
-              k <- k';
-              ko <- Some k;
-              state_map.[(a, i)] <- (role, Observed trace k);
-            }
-          }
-        }
-        | Observed _ _   => { }
-        | IPending _ _   => { }
-        | RPending _ _ _ => { }
-        | Aborted        => { }
-        end;
-      }
-      return ko;
-    }
-  
-    proc test(a, i) = {
-      var role, st, ps, k;
-      var ko <- None;
- 
-      if ((a, i) \in state_map) {
-        (role, st) <- oget state_map.[(a, i)];
-        match st with
-        | Accepted trace k' => {
-          ps <- get_partners (a, i) (Some trace) role state_map;
-          if (card ps <= 1) {
-            ps <- get_observed_partners (a, i) state_map;
-            if (card ps = 0) {
-              if (b0 = false) {
-                k <- k';
-              } else {
-                k <$ dskey;
-              }
-              ko <- Some k;
-              state_map.[(a, i)] <- (role, Observed trace k);
-            }
-          }
-        }
-        | Observed _ _   => { }
-        | IPending _ _   => { }
-        | RPending _ _ _ => { }
-        | Aborted        => { }
-        end;
-      }
-      return ko;
-    }
+    ]
   }
-  
-  proc run() = {
+
+  proc run(b) = {
     var b';
-    WAKE_O.init_mem(false);
-    b' <@ D(WAKE_O).run();
-    return b';
-  }
-}.
-
-module (Red_PRF_ideal (D : A_GWAKE) : A_GPRF) (O : GPRF_out) = {
-  module WAKE_O : GWAKE_out = {
-    var b0 : bool
-
-    var dec_map : ((id * id) * msg_data * ctxt, nonce) fmap
-    var bad : bool
-    var state_map : (id * int, role * instance_state) fmap
-    var psk_map : (id * id, pskey) fmap
-  
-    proc init_mem(b: bool) = {
-      b0 <- b;
-      state_map <- empty;
-      psk_map <- empty;
-      bad <- false;
-      dec_map <- empty;
-    }
-  
-    proc gen_pskey(a, b) = {
-      var k;
-  
-      if ((a, b) \notin psk_map) {
-        k <$ dpskey;
-        psk_map.[a, b] <- k;
-      }
-    }
-  
-    proc send_msg1(a, i, b) = {
-      var ca, mo;
-      
-      mo <- None;
-      if (((a, i) \notin state_map) /\ ((a, b) \in psk_map)) {
-        ca <$ dctxt;
-        bad <- bad \/ exists pk ad, (pk, ad, ca) \in dec_map;
-        if (!bad) {
-          dec_map.[(a, b), msg1_data a b, ca] <- witness;
-          mo <- Some ca;
-          state_map.[a, i] <- (Initiator, IPending (b, witness, witness, ca) (a, ca));
-        }
-      }
-      
-      return mo;
-    }
-
-    proc send_msg2(b : id, j : int, m1 : id * ctxt) : ctxt option = {
-      var a, ca, role, st, cb, mo;
-      
-      mo <- None;
-      (a, ca) <- m1;
-      (role, st) <- oget state_map.[b, j];
-      if (((b, j) \notin state_map) /\ ((a, b) \in psk_map)) {
-        if (dec_map.[(a, b), msg1_data a b, ca] is Some na) {
-          cb <$ dctxt;
-          bad <- bad \/ exists pk ad, (pk, ad, cb) \in dec_map;
-          if (!bad) {
-            dec_map.[(a, b), msg2_data a b ca, cb] <- witness;
-            mo <- Some cb;
-            state_map.[b, j] <- (Responder, RPending (a, witness, witness, witness, ca, cb) m1 cb);
-          }
-        } else {
-          state_map.[b, j] <- (Responder, Aborted);
-        }
-      }
-      
-      return mo;
-    }
-    
-    proc send_msg3(a : id, i : int, m2 : ctxt) : ctxt option = {
-      var role, st, b, psk, na, ca, skey, caf, mo; 
-      
-      mo <- None;
-      if ((a, i) \in state_map) {
-        (role, st) <- oget state_map.[a, i];
-        match (st) with
-        | IPending s m1 => {
-          (b, psk, na, ca) <- s;
-          if (dec_map.[(a, b), msg2_data a b ca, m2] is Some nb) {
-            caf <$ dctxt;
-            bad <- bad \/ exists pk ad, (pk, ad, caf) \in dec_map;
-            if (!bad) {
-              dec_map.[(a, b), msg3_data a b ca m2, caf] <- witness;
-              mo <- Some caf;
-              O.gen((msg3_data a b ca m2, caf));
-              skey <@ O.f((msg3_data a b ca m2, caf), (a, b));
-              state_map.[a, i] <- (Initiator, Accepted ((a, ca), m2, caf) (oget skey));
-            }
-          } else {
-            state_map.[a, i] <- (Initiator, Aborted);
-          }
-        }
-        | RPending _ _ _ => {}
-        | Accepted _ _ => {}
-        | Observed _ _ => {}
-        | Aborted => {}
-        end;
-      }
-      
-      return mo;
-    }
-
-    proc send_fin(b : id, j : int, m3 : ctxt) : unit option = {
-      var role, st, a, psk, na, nb, ca, cb, skey, mo;
-      
-      mo <- None;
-      if ((b, j) \in state_map) {
-        (role, st) <- oget state_map.[b, j];
-        match (st) with
-        | IPending _ _ => {}
-        | RPending s m1 m2 => {
-          (a, psk, na, nb, ca, cb) <- s;
-          if(dec_map.[(a, b), msg3_data a b ca cb, m3] is Some nok) {
-            skey <@ O.f((msg3_data a b ca cb, m3), (a, b));
-            state_map.[b, j] <- (Responder, Accepted ((a, ca), cb, m3) (oget skey));
-            mo <- Some tt;
-          } else {
-           state_map.[b, j] <- (Responder, Aborted);
-          }
-        }
-        | Accepted _ _ => {}
-        | Observed _ _ => {}
-        | Aborted => {}
-        end;
-      }
-      
-      return mo;
-    }
-
-    proc rev_skey(a, i) = {
-      var role, st, ps, k;
-      var ko <- None;
-  
-      if ((a, i) \in state_map) {
-        (role, st) <- oget state_map.[(a, i)];
-        match st with
-        | Accepted trace k' => {
-          ps <- get_partners (a, i) (Some trace) role state_map;
-          if (card ps <= 1) {
-            ps <- get_observed_partners (a, i) state_map;
-            if (card ps = 0) {
-              k <- k';
-              ko <- Some k;
-              state_map.[(a, i)] <- (role, Observed trace k);
-            }
-          }
-        }
-        | Observed _ _   => { }
-        | IPending _ _   => { }
-        | RPending _ _ _ => { }
-        | Aborted        => { }
-        end;
-      }
-      return ko;
-    }
-  
-    proc test(a, i) = {
-      var role, st, ps, k;
-      var ko <- None;
- 
-      if ((a, i) \in state_map) {
-        (role, st) <- oget state_map.[(a, i)];
-        match st with
-        | Accepted trace k' => {
-          ps <- get_partners (a, i) (Some trace) role state_map;
-          if (card ps <= 1) {
-            ps <- get_observed_partners (a, i) state_map;
-            if (card ps = 0) {
-              if (b0 = false) {
-                k <- k';
-              } else {
-                k <$ dskey;
-              }
-              ko <- Some k;
-              state_map.[(a, i)] <- (role, Observed trace k);
-            }
-          }
-        }
-        | Observed _ _   => { }
-        | IPending _ _   => { }
-        | RPending _ _ _ => { }
-        | Aborted        => { }
-        end;
-      }
-      return ko;
-    }
-  }
-  
-  proc run() = {
-    var b';
-    WAKE_O.init_mem(true);
+    WAKE_O.init_mem(b);
     b' <@ D(WAKE_O).run();
     return b';
   }
@@ -883,74 +216,42 @@ clone PROM.FullRO as KROc with
   type in_t    <= trace,
   type out_t   <= skey,
   op   dout  _ <= dskey,
-  type d_in_t  <= unit,
+  type d_in_t  <= bool,
   type d_out_t <= bool
 proof *.
 
-print Game7.
-
-module (Red_ROM_sk_real (D : A_GWAKE) : KROc.RO_Distinguisher) (O : KROc.RO) = {
+module (Red_ROM_sk (D : A_GWAKE) : KROc.RO_Distinguisher) (R : KROc.RO) = {
   module WAKE_O : GWAKE_out = Game7 with {
     proc send_msg3 [
       ^if.^match#IPending.^match#Some.^if.^skey<$ ~ {
-        O.sample(((a, ca), m2, caf));
+        R.sample(((a, ca), m2, caf));
         skey <- witness;
       }
     ]
 
     proc rev_skey [
-      ^if.^match#Accepted.^if.^if.^k<- ~ { k <@ O.get(trace); }
+      ^if.^match#Accepted.^if.^if.^k<- ~ { k <@ R.get(trace); }
     ]
 
     proc test [
-      ^if.^match#Accepted.^if.^if.^if.^k<- ~ { k <@ O.get(trace); }
-      ^if.^match#Accepted.^if.^if.^if?^k<$ + ^ { k <@ O.get(trace); }
+      ^if.^match#Accepted.^if.^if.^if ~ { k <@ R.get(trace); if (b0) {k <$ dskey; }}
     ]
   }
 
-  proc distinguish() = {
+  proc distinguish(b) = {
     var b';
-    WAKE_O.init_mem(false);
+    WAKE_O.init_mem(b);
     b' <@ D(WAKE_O).run();
     return b';
   }
 }.
-
-module (Red_ROM_sk_ideal (D : A_GWAKE) : KROc.RO_Distinguisher) (O : KROc.RO) = {
-  module WAKE_O : GWAKE_out = Game7 with {
-    proc send_msg3 [
-      ^if.^match#IPending.^match#Some.^if.^skey<$ ~ {
-        O.sample(((a, ca), m2, caf));
-        skey <- witness;
-      }
-    ]
-
-    proc rev_skey [
-      ^if.^match#Accepted.^if.^if.^k<- ~ { k <@ O.get(trace); }
-    ]
-
-    proc test [
-      ^if.^match#Accepted.^if.^if.^if?^k<$ + ^ { k <@ O.get(trace); }
-      ^if.^match#Accepted.^if.^if.^if.^k<- ~ { k <@ O.get(trace); }
-    ]
-  }
-
-  proc distinguish() = {
-    var b';
-    WAKE_O.init_mem(true);
-    b' <@ D(WAKE_O).run();
-    return b';
-  }
-}.
-
-print Red_ROM_sk_real.WAKE_O.
 
 (* ------------------------------------------------------------------------------------------ *)
 (* Security Proof *)
 (* ------------------------------------------------------------------------------------------ *)
 section.
 
-declare module A <: A_GWAKE {-GWAKEb, -Game1, -Game2, -Game3, -Game4, -Game5, -Game6, -Game7, -Game8, -GAEAD0, -GAEAD1, -PRF0, -PRF1, -Red_AEAD_real, -Red_AEAD_ideal, -Red_Coll_real, -Red_Coll_ideal, -Red_ROM_real, -Red_ROM_ideal, -Red_PRF_real, -Red_PRF_ideal, -RO, -FRO, -BD.Sample, -KROc.RO, -KROc.FRO, -Red_ROM_sk_real, -Red_ROM_sk_ideal}.
+declare module A <: A_GWAKE {-GWAKEb, -Game1, -Game2, -Game3, -Game4, -Game5, -Game6, -Game7, -Game8, -GAEAD0, -GAEAD1, -PRF0, -PRF1, -Red_AEAD, -Red_Coll_real, -Red_Coll_ideal, -Red_ROM, -Red_PRF, -NROc.RO, -NROc.FRO, -BD.Sample, -KROc.RO, -KROc.FRO, -Red_ROM_sk}.
 
 declare axiom A_ll:
 forall (GW <: GWAKE_out{-A}),
@@ -963,12 +264,12 @@ forall (GW <: GWAKE_out{-A}),
 
 declare axiom A_bounded_qs: forall (GW <: GWAKE_out{-A}), hoare[A(Counter(GW)).run: Counter.cm1 = 0 /\ Counter.cm2 = 0 /\ Counter.cm3 = 0 ==> Counter.cm1 <= q_m1 /\ Counter.cm2 <= q_m2 /\ Counter.cm3 <= q_m3].
 
+(*
 lemma obs_ps sm h h' s:
     get_as_Observed s = None =>
     (get_observed_partners h sm.[h' <- ((fst (oget sm.[h'])), s)]) = get_observed_partners h sm.
 proof.
 admitted.
-
 
 (* ------------------------------------------------------------------------------------------ *)
 (* Step 8: Relating real and ideal side *)
@@ -986,28 +287,26 @@ call (: ={state_map, psk_map, dec_map, bad, prfkey_map, sk_map}(Game8, Game8) /\
   move => tr sk.
   sp; if => //. smt().
   sp; if => //.
-  rcondt{1} ^if; 1: by auto.
-  rcondf{2} ^if; 1: by auto.
   auto => /#.
 
 auto => />.
 qed. 
+*)
 
 (* ------------------------------------------------------------------------------------------ *)
 (* Step 7: Delaying sampling of the keys *)
-lemma Step7 bit &m:
-    Pr[E_GWAKE(Game7, A).run(bit) @ &m : res] = Pr[E_GWAKE(Game8, A).run(bit) @ &m : res].
+lemma Step7 &m:
+    Pr[E_GWAKE(Game7, A).run(false) @ &m : res] = Pr[E_GWAKE(Game7, A).run(true) @ &m : res].
 proof.
 byequiv => //.
 proc*.
 
-case (bit).
-
-(* Proof for the ideal side *)
-transitivity* {1} { r <@ KROc.MainD(Red_ROM_sk_ideal(A), KROc.RO).distinguish(); }.
+(* Proof for the real side *)
+transitivity* {1} { r <@ KROc.MainD(Red_ROM_sk(A), KROc.RO).distinguish(false); }.
 + inline*; wp.
-  call(: ={b0, state_map, psk_map, dec_map, bad, prfkey_map}(Game7, Red_ROM_sk_ideal.WAKE_O)
+  call(: ={b0, state_map, psk_map, dec_map, bad, prfkey_map}(Game7, Red_ROM_sk.WAKE_O)
          /\ Game7.sk_map{1} = KROc.RO.m{2}
+         /\ !Game7.b0{1}
   /\ (forall h r tr k, Game7.state_map.[h] = Some (r, Accepted tr k) => tr \in Game7.sk_map){1}
   /\ (forall a b m1 m2 m3, ((a, b), msg3_data a b m1 m2, m3) \in Game7.dec_map => ((a, m1), m2, m3) \in Game7.sk_map){1}
   /\ (forall m1 m2 m3, (forall pk ad, (pk, ad, m3) \notin Game7.dec_map) => (m1, m2, m3) \notin Game7.sk_map){1}
@@ -1069,25 +368,152 @@ transitivity* {1} { r <@ KROc.MainD(Red_ROM_sk_ideal(A), KROc.RO).distinguish();
 
   - proc; inline*. 
     sp; wp ^if ^if; if => //.
-    sp 1 1. admit. (*match = => //.
+    sp 1 1; match = => //.
     + smt().
     move=> tr k'.
     sp ^if & -1 ^if & -1; if => //.
     + smt().
     sp ^if & -1 ^if & -1; if=> //.
-    if => //.
-    + auto=> /> &1 &2.
-      smt(get_setE).
-    auto => />.
-    smt(get_setE).*)
-  
+    rcondt {1} ^if; 1: by auto => />.
+    rcondf {2} ^if{2}; 1: by auto.
+    auto=> /> &1 &2.
+    smt(get_setE).
+
   auto=> />.
   smt(emptyE).
 
-rewrite equiv [{1} 1 (KROc.FullEager.RO_LRO (Red_ROM_sk_ideal(A)) _)]; 1: by move=> _; exact dskey_ll.
-inline*; wp.
-call(: ={b0, state_map, psk_map, dec_map, bad, prfkey_map}(Red_ROM_sk_ideal.WAKE_O, Game8)
-       /\ (Game8.sk_map{2} = KROc.RO.m{1})
+rewrite equiv [{1} 1 (KROc.FullEager.RO_LRO (Red_ROM_sk(A)) _)]; 1: by move=> _; exact dskey_ll.
+
+(* Proof for the ideal side *)
+symmetry.
+transitivity* {1} { r <@ KROc.MainD(Red_ROM_sk(A), KROc.RO).distinguish(true); }.
++ inline*; wp.
+  call(: ={b0, state_map, psk_map, dec_map, bad, prfkey_map}(Game7, Red_ROM_sk.WAKE_O)
+         /\ Game7.sk_map{1} = KROc.RO.m{2}
+         /\ Game7.b0{1}
+  /\ (forall h r tr k, Game7.state_map.[h] = Some (r, Accepted tr k) => tr \in Game7.sk_map){1}
+  /\ (forall a b m1 m2 m3, ((a, b), msg3_data a b m1 m2, m3) \in Game7.dec_map => ((a, m1), m2, m3) \in Game7.sk_map){1}
+  /\ (forall m1 m2 m3, (forall pk ad, (pk, ad, m3) \notin Game7.dec_map) => (m1, m2, m3) \notin Game7.sk_map){1}
+  ).
+  
+  - by sim />.  
+
+  - proc; inline*. 
+    sp; wp; if => //.
+    auto => />.
+    smt(mem_set get_setE).
+  
+  - proc; inline*.
+    sp; wp; if => //.
+    match = => //.
+    + auto => />. 
+      smt(get_setE).
+    auto => />.
+    smt(mem_set get_setE).
+  
+  - proc; inline*.
+    sp; wp; if=> //. 
+    sp; match = => //.
+    + smt().  
+    move=> s m1.
+    sp; match =.
+    + smt().
+    + auto=> />.
+      smt(get_setE).
+    move=> nb.
+    seq 1 1 : (#pre /\ ={caf}); 1: by auto.
+    sp; if=> //.
+    auto=> />.
+    smt(mem_set get_setE).
+  
+  - proc; inline*.
+    sp; wp ^if ^if; if=> //. 
+    sp; match = => //.
+    + smt().
+    move=> s m1 m2. 
+    sp; match =.
+    + smt().
+    + auto=> />.
+      smt(get_setE).
+    move=> nok.
+    auto=> />.
+    smt(get_setE).
+
+  - proc; inline*. 
+    sp; wp ^if ^if; if => //.
+    sp; match = => //.
+    + smt().
+    move=> tr k'.
+    sp ^if & -1 ^if & -1; if => //.
+    + smt().
+    sp ^if & -1 ^if & -1; if=> //.
+    auto=> /> &1 &2.
+    smt(get_setE).
+
+  - proc; inline*. 
+    sp; wp ^if ^if; if => //.
+    sp 1 1; match = => //.
+    + smt().
+    move=> tr k'.
+    sp ^if & -1 ^if & -1; if => //.
+    + smt().
+    sp ^if & -1 ^if & -1; if=> //.
+    rcondf {1} ^if; 1: by auto => />.
+    rcondt {2} ^if{2}; 1: by auto.
+    auto=> /> &1 &2.
+    smt(get_setE).
+
+  auto=> />.
+  smt(emptyE).
+
+rewrite equiv [{1} 1 (KROc.FullEager.RO_LRO (Red_ROM_sk(A)) _)]; 1: by move=> _; exact dskey_ll.
+inline; wp.
+call(: ={state_map, psk_map, dec_map, bad, prfkey_map, sk_map}(Red_ROM_sk.WAKE_O, Red_ROM_sk.WAKE_O)
+     /\ Red_ROM_sk.WAKE_O.b0{1}
+     /\ !Red_ROM_sk.WAKE_O.b0{2}
+     /\ (forall h, h \in KROc.RO.m{1} <=> h \in KROc.RO.m{2})
+); 1..5: by sim />.
+- proc.
+  sp; if => //.
+  sp; match = => //.
+  + smt().
+  move => tr k'.
+  sp ^if & -1 ^if & -1; if => //.
+  + smt().
+  sp ^if & -1 ^if & -1; if => //.
+  inline.
+  rcondt {1} ^if.
+  + auto => />.
+    admit. (* INV: No observed partners => no key stored yet *)
+  rcondt {2} ^if.
+  + admit. (* trivial from inv and above *)
+  auto => />.
+  smt(mem_set get_setE).
+
+- proc.
+  sp; if => //.
+  sp; match = => //.
+  + smt().
+  move => tr k'.
+  sp ^if & -1 ^if & -1; if => //.
+  + smt().
+  sp ^if & -1 ^if & -1; if => //.
+  inline.
+  rcondt {1} ^if.
+  + auto => />.
+    admit. (* INV: No observed partners => no key stored yet *)
+  rcondt {2} ^if.
+  + admit. (* trivial from inv and above *)
+  rcondt {1} ^if; 1: by auto.
+  rcondf {2} ^if; 1: by auto.
+  auto => />.
+  smt(get_setE mem_set).
+
+auto => />.
+qed.
+
+(*
+call(: ={b0, state_map, psk_map, dec_map, bad, prfkey_map, sk_map}(Red_ROM_sk.WAKE_O, Game8)
 /\ (forall h r tr k, Game8.state_map{2}.[h] = Some (r, Accepted tr k) => tr \in Game8.sk_map{2})
 /\ (forall a b m1 m2 m3, ((a, b), msg3_data a b m1 m2, m3) \in Game8.dec_map => ((a, m1), m2, m3) \in Game8.sk_map){2}
 /\ (forall m1 m2 m3, (forall pk ad, (pk, ad, m3) \notin Game8.dec_map) => (m1, m2, m3) \notin Game8.sk_map){2}
@@ -1121,7 +547,6 @@ call(: ={b0, state_map, psk_map, dec_map, bad, prfkey_map}(Red_ROM_sk_ideal.WAKE
   seq 1 1 : (#pre /\ ={caf}); 1: by auto.
   sp; if=> //.
   auto=> /> &1 &2 *.
-  split. admit.
   smt(get_setE mem_set).
 
 - proc; inline*.
@@ -1147,6 +572,7 @@ call(: ={b0, state_map, psk_map, dec_map, bad, prfkey_map}(Red_ROM_sk_ideal.WAKE
   sp ^if & -1 ^if & -1; if=> //.
   auto=> /> &1 &2 *.
   split. smt(get_setE mem_set).
+  move => *.
   admit.
 
 - proc; inline*.
@@ -1157,18 +583,19 @@ call(: ={b0, state_map, psk_map, dec_map, bad, prfkey_map}(Red_ROM_sk_ideal.WAKE
   sp ^if & -1 ^if & -1; if => //.
   + smt().
   sp ^if & -1 ^if & -1; if=> //.
-  if => //.
+  case (Red_ROM_sk.WAKE_O.b0{1}).
+  + rcondt {1} ^if{2}; 1: by auto.
     auto => /> &1 &2 *.
-    split. smt(get_setE mem_set). 
-    admit.
+    smt(get_setE mem_set). 
+  rcondf {1} ^if{2}; 1: by auto.
   auto => /> &1 &2 *.
-  smt(get_setE mem_set).
+  split. smt(get_setE mem_set).
+  admit.
 
 auto=> />.
 smt(emptyE).
-
-admit. (* Repeat on the real side *)
 qed.
+*)
 
 (* ------------------------------------------------------------------------------------------ *)
 (* Step 0: Inline procedure calls, and remove pskeys from the state using psk_map to retrieve. *)
@@ -1386,10 +813,10 @@ qed.
 (* ------------------------------------------------------------------------------------------ *)
 (* Step 1: Apply the AEAD assumption. *)
 
-lemma Step1_real &m:
-    `|Pr[E_GWAKE(Game1, A).run(false) @ &m : res] - Pr[E_GWAKE(Game2, A).run(false) @ &m : res]|
+lemma Step1 bit &m:
+    `|Pr[E_GWAKE(Game1, A).run(bit) @ &m : res] - Pr[E_GWAKE(Game2, A).run(bit) @ &m : res]|
   = 
-    `|Pr[E_GAEAD(GAEAD0, Red_AEAD_real(A)).run() @ &m : res] - Pr[E_GAEAD(GAEAD1, Red_AEAD_real(A)).run() @ &m : res]|.
+    `|Pr[E_GAEAD(GAEAD0, Red_AEAD(A)).run(bit) @ &m : res] - Pr[E_GAEAD(GAEAD1, Red_AEAD(A)).run(bit) @ &m : res]|.
 proof.
 do! congr.
 + byequiv => //.
@@ -1397,19 +824,19 @@ do! congr.
   wp.
   call (:
         ={psk_map}(Game1, GAEADb)
-     /\ ={b0, state_map}(Game1, Red_AEAD_real.WAKE_O)
+     /\ ={b0, state_map}(Game1, Red_AEAD.WAKE_O)
      /\ (forall a i, Game1_inv Game1.state_map Game1.psk_map a i){1}
   )=> //.
 
   - conseq (: ={res}
          /\ ={psk_map}(Game1, GAEADb)
-         /\ ={b0, state_map}(Game1, Red_AEAD_real.WAKE_O)
+         /\ ={b0, state_map}(Game1, Red_AEAD.WAKE_O)
     ) Game1_inv_gen_pskey _ => //.
-    by proc; if; auto.
+    by proc; inline; sp; if; auto.
 
   - conseq (: ={res}
          /\ ={psk_map}(Game1, GAEADb)
-         /\ ={b0, state_map}(Game1, Red_AEAD_real.WAKE_O)
+         /\ ={b0, state_map}(Game1, Red_AEAD.WAKE_O)
     ) Game1_inv_send_msg1 _ => //.
     proc; inline.
     sp; wp; if=> //.
@@ -1417,7 +844,7 @@ do! congr.
 
   - conseq (: ={res}
          /\ ={psk_map}(Game1, GAEADb)
-         /\ ={b0, state_map}(Game1, Red_AEAD_real.WAKE_O)
+         /\ ={b0, state_map}(Game1, Red_AEAD.WAKE_O)
     ) Game1_inv_send_msg2 _ => //.
     proc; inline.
     sp; wp; if=> //.
@@ -1431,7 +858,7 @@ do! congr.
 
   - conseq (: ={res}
          /\ ={psk_map}(Game1, GAEADb)
-         /\ ={b0, state_map}(Game1, Red_AEAD_real.WAKE_O)
+         /\ ={b0, state_map}(Game1, Red_AEAD.WAKE_O)
     ) Game1_inv_send_msg3 _ => //.
     proc; inline.
     sp; wp; if=> //.
@@ -1452,7 +879,7 @@ do! congr.
 
   - conseq (: ={res}
          /\ ={psk_map}(Game1, GAEADb)
-         /\ ={b0, state_map}(Game1, Red_AEAD_real.WAKE_O)
+         /\ ={b0, state_map}(Game1, Red_AEAD.WAKE_O)
     ) Game1_inv_send_fin _ => //.
     proc; inline.
     sp; wp ^if ^if; if=> //.
@@ -1467,13 +894,13 @@ do! congr.
 
   - conseq (: ={res}
          /\ ={psk_map}(Game1, GAEADb)
-         /\ ={b0, state_map}(Game1, Red_AEAD_real.WAKE_O)
+         /\ ={b0, state_map}(Game1, Red_AEAD.WAKE_O)
     ) Game1_inv_rev_skey _ => //.
     by sim.
 
   - conseq (: ={res}
          /\ ={psk_map}(Game1, GAEADb)
-         /\ ={b0, state_map}(Game1, Red_AEAD_real.WAKE_O)
+         /\ ={b0, state_map}(Game1, Red_AEAD.WAKE_O)
     ) Game1_inv_test _ => //.
     by sim. 
   
@@ -1486,21 +913,21 @@ proc; inline*.
 wp.
 call (:
       ={psk_map}(Game2, GAEADb)
-      /\ ={b0, state_map}(Game2, Red_AEAD_real.WAKE_O)
+      /\ ={b0, state_map}(Game2, Red_AEAD.WAKE_O)
       /\ Game2.dec_map{1} = GAEAD1.ctxts{2}
       /\ (forall a i, Game1_inv Game2.state_map Game2.psk_map a i){1}
 ).
 - conseq (: ={res}
        /\ ={psk_map}(Game2, GAEADb)
-       /\ ={b0, state_map}(Game2, Red_AEAD_real.WAKE_O)
+       /\ ={b0, state_map}(Game2, Red_AEAD.WAKE_O)
        /\ Game2.dec_map{1} = GAEAD1.ctxts{2}
   ) Game2_inv_gen_pskey _ => //.
-  proc.
+  proc; inline; sp.
   by if; auto.
 
 - conseq (: ={res}
        /\ ={psk_map}(Game2, GAEADb)
-       /\ ={b0, state_map}(Game2, Red_AEAD_real.WAKE_O)
+       /\ ={b0, state_map}(Game2, Red_AEAD.WAKE_O)
        /\ Game2.dec_map{1} = GAEAD1.ctxts{2}
   ) Game2_inv_send_msg1 _ => //.
   proc; inline.
@@ -1511,7 +938,7 @@ call (:
 
 - conseq (: ={res}
        /\ ={psk_map}(Game2, GAEADb)
-       /\ ={b0, state_map}(Game2, Red_AEAD_real.WAKE_O)
+       /\ ={b0, state_map}(Game2, Red_AEAD.WAKE_O)
        /\ Game2.dec_map{1} = GAEAD1.ctxts{2}
   ) Game2_inv_send_msg2 _ => //.
   proc; inline.
@@ -1526,7 +953,7 @@ call (:
 
 - conseq (: ={res}
        /\ ={psk_map}(Game2, GAEADb)
-       /\ ={b0, state_map}(Game2, Red_AEAD_real.WAKE_O)
+       /\ ={b0, state_map}(Game2, Red_AEAD.WAKE_O)
        /\ Game2.dec_map{1} = GAEAD1.ctxts{2}
   ) Game2_inv_send_msg3 _ => //.
   proc; inline.
@@ -1551,7 +978,7 @@ call (:
 
 - conseq (: ={res}
        /\ ={psk_map}(Game2, GAEADb)
-       /\ ={b0, state_map}(Game2, Red_AEAD_real.WAKE_O)
+       /\ ={b0, state_map}(Game2, Red_AEAD.WAKE_O)
        /\ Game2.dec_map{1} = GAEAD1.ctxts{2}
   ) Game2_inv_send_fin _ => //.
   proc; inline.
@@ -1567,211 +994,14 @@ call (:
 
 - conseq (: ={res}
        /\ ={psk_map}(Game2, GAEADb)
-       /\ ={b0, state_map}(Game2, Red_AEAD_real.WAKE_O)
+       /\ ={b0, state_map}(Game2, Red_AEAD.WAKE_O)
        /\ Game2.dec_map{1} = GAEAD1.ctxts{2}
   ) Game2_inv_rev_skey _ => //.
   by sim.
 
 - conseq (: ={res}
        /\ ={psk_map}(Game2, GAEADb)
-       /\ ={b0, state_map}(Game2, Red_AEAD_real.WAKE_O)
-       /\ Game2.dec_map{1} = GAEAD1.ctxts{2}
-  ) Game2_inv_test _ => //.
-  by sim.
-
-auto=> /> a i.
-exact /Game1_undef/emptyE.
-qed.
-
-lemma Step1_ideal &m:
-    `|Pr[E_GWAKE(Game1, A).run(true) @ &m : res] - Pr[E_GWAKE(Game2, A).run(true) @ &m : res]|
-  = 
-    `|Pr[E_GAEAD(GAEAD0, Red_AEAD_ideal(A)).run() @ &m : res] - Pr[E_GAEAD(GAEAD1, Red_AEAD_ideal(A)).run() @ &m : res]|.
-proof.
-do! congr.
-+ byequiv => //.
-  proc; inline*.
-  wp.
-  call (:
-        ={psk_map}(Game1, GAEADb)
-     /\ ={b0, state_map}(Game1, Red_AEAD_ideal.WAKE_O)
-     /\ (forall a i, Game1_inv Game1.state_map Game1.psk_map a i){1}
-  )=> //.
-
-  - conseq (: ={res}
-         /\ ={psk_map}(Game1, GAEADb)
-         /\ ={b0, state_map}(Game1, Red_AEAD_ideal.WAKE_O)
-    ) Game1_inv_gen_pskey _ => //.
-    by proc; if; auto.
-
-  - conseq (: ={res}
-         /\ ={psk_map}(Game1, GAEADb)
-         /\ ={b0, state_map}(Game1, Red_AEAD_ideal.WAKE_O)
-    ) Game1_inv_send_msg1 _ => //.
-    proc; inline.
-    sp; wp; if=> //.
-    by match Some {2} ^match; auto; smt().
-
-  - conseq (: ={res}
-         /\ ={psk_map}(Game1, GAEADb)
-         /\ ={b0, state_map}(Game1, Red_AEAD_ideal.WAKE_O)
-    ) Game1_inv_send_msg2 _ => //.
-    proc; inline.
-    sp; wp; if=> //.
-    match Some {2} ^match.
-    + auto; smt().
-    sp; match =.
-    + by move=> /> /#.
-    + by auto. 
-    move=> na.
-    by match Some {2} ^match; auto; smt().
-
-  - conseq (: ={res}
-         /\ ={psk_map}(Game1, GAEADb)
-         /\ ={b0, state_map}(Game1, Red_AEAD_ideal.WAKE_O)
-    ) Game1_inv_send_msg3 _ => //.
-    proc; inline.
-    sp; wp; if=> //.
-    sp; match = => //. 
-    + smt().
-    move=> st m1.
-    exlim Game1.state_map{1}, Game1.psk_map{1}, a{1}, i{1} => sm pm a i.
-    case @[ambient] _: (forall a i, Game1_inv sm pm a i) => [inv|?]; 2: by exfalso => /#. 
-    case @[ambient] _: (inv a i); 1,2,4,5,6: (move=> *; exfalso=> /#).
-    move=> b na c1 kab smai pmab.
-    match Some {2} ^match; 1: by auto=> /#.
-    sp; match =.
-    + by auto=> /> /#. 
-    + by auto=> /> /#.
-    move=> nb.
-    match Some {2} ^match; 1: by auto=> /#.
-    by auto=> /> /#.
-
-  - conseq (: ={res}
-         /\ ={psk_map}(Game1, GAEADb)
-         /\ ={b0, state_map}(Game1, Red_AEAD_ideal.WAKE_O)
-    ) Game1_inv_send_fin _ => //.
-    proc; inline.
-    sp; wp ^if ^if; if=> //.
-    sp; match = => //.
-    + move=> /#.
-    move=> st m1 m2.
-    match Some {2} ^match.
-    + auto=> />. 
-      move=> &hr smr sml invl bj_in.
-      by case: (invl b{m0} j{m0})=> /#.
-    by sp; match =; auto=> /> /#.
-
-  - conseq (: ={res}
-         /\ ={psk_map}(Game1, GAEADb)
-         /\ ={b0, state_map}(Game1, Red_AEAD_ideal.WAKE_O)
-    ) Game1_inv_rev_skey _ => //.
-    by sim.
-
-  - conseq (: ={res}
-         /\ ={psk_map}(Game1, GAEADb)
-         /\ ={b0, state_map}(Game1, Red_AEAD_ideal.WAKE_O)
-    ) Game1_inv_test _ => //.
-    by sim. 
-  
-  auto=> />.
-  move=> a i.
-  exact /Game1_undef/emptyE.
-
-byequiv => //.
-proc; inline*.
-wp.
-call (:
-      ={psk_map}(Game2, GAEADb)
-      /\ ={b0, state_map}(Game2, Red_AEAD_ideal.WAKE_O)
-      /\ Game2.dec_map{1} = GAEAD1.ctxts{2}
-      /\ (forall a i, Game1_inv Game2.state_map Game2.psk_map a i){1}
-).
-- conseq (: ={res}
-       /\ ={psk_map}(Game2, GAEADb)
-       /\ ={b0, state_map}(Game2, Red_AEAD_ideal.WAKE_O)
-       /\ Game2.dec_map{1} = GAEAD1.ctxts{2}
-  ) Game2_inv_gen_pskey _ => //.
-  proc.
-  by if; auto.
-
-- conseq (: ={res}
-       /\ ={psk_map}(Game2, GAEADb)
-       /\ ={b0, state_map}(Game2, Red_AEAD_ideal.WAKE_O)
-       /\ Game2.dec_map{1} = GAEAD1.ctxts{2}
-  ) Game2_inv_send_msg1 _ => //.
-  proc; inline.
-  sp; wp; if=> //.
-  rcondt{2} ^if; 1: by auto.
-  swap {2} ^c<$ @ ^na<$.
-  by auto.
-
-- conseq (: ={res}
-       /\ ={psk_map}(Game2, GAEADb)
-       /\ ={b0, state_map}(Game2, Red_AEAD_ideal.WAKE_O)
-       /\ Game2.dec_map{1} = GAEAD1.ctxts{2}
-  ) Game2_inv_send_msg2 _ => //.
-  proc; inline.
-  sp; wp; if=> //.
-  rcondt {2} 5; 1: by auto.
-  sp; match = => //.
-  + by auto.
-  move=> na.
-  rcondt {2} ^if; 1: by auto.
-  swap {2} ^c0<$ @ ^nb<$.
-  by auto.
-
-- conseq (: ={res}
-       /\ ={psk_map}(Game2, GAEADb)
-       /\ ={b0, state_map}(Game2, Red_AEAD_ideal.WAKE_O)
-       /\ Game2.dec_map{1} = GAEAD1.ctxts{2}
-  ) Game2_inv_send_msg3 _ => //.
-  proc; inline.
-  sp; wp; if=> //.
-  sp; match = => //.
-  + smt().
-  move=> st m1.
-  rcondt {2} ^if.
-  + auto=> />.
-    move=> &hr smr sml invl ai_in.
-    by case: (invl a{m0} i{m0})=> /#.
-  sp; match =.
-  + by auto.
-  + by auto.
-  move=> nb.
-  rcondt {2} ^if.
-  + auto=> />.
-    move=> &hr decl decr smr sml invl ai_in ok _.
-    by case: (invl a{m0} i{m0})=> /#.
-  swap {2} ^c0<$ @ ^ok<$.
-  by auto.
-
-- conseq (: ={res}
-       /\ ={psk_map}(Game2, GAEADb)
-       /\ ={b0, state_map}(Game2, Red_AEAD_ideal.WAKE_O)
-       /\ Game2.dec_map{1} = GAEAD1.ctxts{2}
-  ) Game2_inv_send_fin _ => //.
-  proc; inline.
-  sp; wp ^if ^if; if=> //.
-  sp; match = => //.
-  + smt().
-  move=> st m1 m2.
-  rcondt {2} 6.
-  + auto=> />.
-    move=> &hr smr sml invl ai_in.
-    by case: (invl b{m0} j{m0})=> /#.
-  by sp; match =; auto.
-
-- conseq (: ={res}
-       /\ ={psk_map}(Game2, GAEADb)
-       /\ ={b0, state_map}(Game2, Red_AEAD_ideal.WAKE_O)
-       /\ Game2.dec_map{1} = GAEAD1.ctxts{2}
-  ) Game2_inv_rev_skey _ => //.
-  by sim.
-
-- conseq (: ={res}
-       /\ ={psk_map}(Game2, GAEADb)
-       /\ ={b0, state_map}(Game2, Red_AEAD_ideal.WAKE_O)
+       /\ ={b0, state_map}(Game2, Red_AEAD.WAKE_O)
        /\ Game2.dec_map{1} = GAEAD1.ctxts{2}
   ) Game2_inv_test _ => //.
   by sim.
@@ -2284,16 +1514,13 @@ proof *.
 lemma Step4 bit &m: Pr[E_GWAKE(Game4, A).run(bit) @ &m : res] = Pr[E_GWAKE(Game5, A).run(bit) @ &m : res].
 byequiv => //.
 proc*.
-case (bit).
-
-(* Proof for the ideal side *)
-transitivity* {1} { r <@ MainD(Red_ROM_ideal(A), RO).distinguish(); }.
+transitivity* {1} { r <@ NROc.MainD(Red_ROM(A), NROc.RO).distinguish(b); }.
 
 + inline*.
   wp.
-  call (: ={b0, state_map, psk_map, bad}(Game4, Red_ROM_ideal.WAKE_O)
-       /\ (forall h, h \in Game4.dec_map{1} <=> h \in Red_ROM_ideal.WAKE_O.dec_map{2})
-       /\ (forall c ad n, (exists pk, Game4.dec_map{1}.[(pk, ad, c)] = Some n) <=> RO.m{2}.[(ad, c)] = Some n)
+  call (: ={b0, state_map, psk_map, bad}(Game4, Red_ROM.WAKE_O)
+       /\ (forall h, h \in Game4.dec_map{1} <=> h \in Red_ROM.WAKE_O.dec_map{2})
+       /\ (forall c ad n, (exists pk, Game4.dec_map{1}.[(pk, ad, c)] = Some n) <=> NROc.RO.m{2}.[(ad, c)] = Some n)
        /\ (forall a b ca cb, ((a, b), msg2_data a b ca, cb) \in Game4.dec_map => ((a, b), msg1_data a b, ca) \in Game4.dec_map){1}
        /\ (forall a b ca cb caf, ((a, b), msg3_data a b ca cb, caf) \in Game4.dec_map => ((a, b), msg2_data a b ca, cb) \in Game4.dec_map){1}
   ) => //.
@@ -2368,63 +1595,63 @@ transitivity* {1} { r <@ MainD(Red_ROM_ideal(A), RO).distinguish(); }.
    auto=> />.
    smt(emptyE).
   
-rewrite equiv [{1} 1 (FullEager.RO_LRO (Red_ROM_ideal(A)) _)]; 1: by move=> _; exact dnonce_ll.
+rewrite equiv [{1} 1 (NROc.FullEager.RO_LRO (Red_ROM(A)) _)]; 1: by move=> _; exact dnonce_ll.
 inline*.
 wp; call (: 
-  ={b0, state_map, psk_map, bad, dec_map}(Red_ROM_ideal.WAKE_O, Game5)
+  ={b0, state_map, psk_map, bad, dec_map}(Red_ROM.WAKE_O, Game5)
   /\ (forall a b ca, (forall cb caf, (msg3_data a b ca cb, caf) \notin Game5.prfkey_map{2})
-        => (msg1_data a b, ca) \notin RO.m{1})
+        => (msg1_data a b, ca) \notin NROc.RO.m{1})
   /\ (forall a b ca cb, (forall caf, (msg3_data a b ca cb, caf) \notin Game5.prfkey_map{2})
-        => (msg2_data a b ca, cb) \notin RO.m{1})
+        => (msg2_data a b ca, cb) \notin NROc.RO.m{1})
   /\ (forall a b ca cb caf, (msg3_data a b ca cb, caf) \in Game5.prfkey_map{2} =>
          exists na nb, Game5.prfkey_map{2}.[(msg3_data a b ca cb, caf)] = Some (na, nb) /\
-                       RO.m{1}.[(msg1_data a b, ca)] = Some na /\
-                       RO.m{1}.[(msg2_data a b ca, cb)] = Some nb)
+                       NROc.RO.m{1}.[(msg1_data a b, ca)] = Some na /\
+                       NROc.RO.m{1}.[(msg2_data a b ca, cb)] = Some nb)
   /\ (Game5_inv_full Game5.state_map Game5.dec_map Game5.prfkey_map){2}
 ) => //.
 
 - by sim />.
 
 - conseq (: ={res}
-  /\ ={b0, state_map, psk_map, bad, dec_map}(Red_ROM_ideal.WAKE_O, Game5)
+  /\ ={b0, state_map, psk_map, bad, dec_map}(Red_ROM.WAKE_O, Game5)
   /\ (forall a b ca, (forall cb caf, (msg3_data a b ca cb, caf) \notin Game5.prfkey_map{2})
-        => (msg1_data a b, ca) \notin RO.m{1})
+        => (msg1_data a b, ca) \notin NROc.RO.m{1})
   /\ (forall a b ca cb, (forall caf, (msg3_data a b ca cb, caf) \notin Game5.prfkey_map{2})
-        => (msg2_data a b ca, cb) \notin RO.m{1})
+        => (msg2_data a b ca, cb) \notin NROc.RO.m{1})
   /\ (forall a b ca cb caf, (msg3_data a b ca cb, caf) \in Game5.prfkey_map{2} =>
          exists na nb, Game5.prfkey_map{2}.[(msg3_data a b ca cb, caf)] = Some (na, nb) /\
-                       RO.m{1}.[(msg1_data a b, ca)] = Some na /\
-                       RO.m{1}.[(msg2_data a b ca, cb)] = Some nb)
+                       NROc.RO.m{1}.[(msg1_data a b, ca)] = Some na /\
+                       NROc.RO.m{1}.[(msg2_data a b ca, cb)] = Some nb)
   ) _ Game5_inv_send_msg1 => //.
   proc; inline*.
   sp; wp; if=> //.
   by auto=> />.
 
 - conseq (: ={res}
-  /\ ={b0, state_map, psk_map, bad, dec_map}(Red_ROM_ideal.WAKE_O, Game5)
+  /\ ={b0, state_map, psk_map, bad, dec_map}(Red_ROM.WAKE_O, Game5)
   /\ (forall a b ca, (forall cb caf, (msg3_data a b ca cb, caf) \notin Game5.prfkey_map{2})
-        => (msg1_data a b, ca) \notin RO.m{1})
+        => (msg1_data a b, ca) \notin NROc.RO.m{1})
   /\ (forall a b ca cb, (forall caf, (msg3_data a b ca cb, caf) \notin Game5.prfkey_map{2})
-        => (msg2_data a b ca, cb) \notin RO.m{1})
+        => (msg2_data a b ca, cb) \notin NROc.RO.m{1})
   /\ (forall a b ca cb caf, (msg3_data a b ca cb, caf) \in Game5.prfkey_map{2} =>
          exists na nb, Game5.prfkey_map{2}.[(msg3_data a b ca cb, caf)] = Some (na, nb) /\
-                       RO.m{1}.[(msg1_data a b, ca)] = Some na /\
-                       RO.m{1}.[(msg2_data a b ca, cb)] = Some nb)
+                       NROc.RO.m{1}.[(msg1_data a b, ca)] = Some na /\
+                       NROc.RO.m{1}.[(msg2_data a b ca, cb)] = Some nb)
   ) _ Game5_inv_send_msg2 => //.
   proc; inline*.
   sp; wp; if=> //.
   by sp; match =; auto=> />.
 
 - conseq (: ={res}
-  /\ ={b0, state_map, psk_map, bad, dec_map}(Red_ROM_ideal.WAKE_O, Game5)
+  /\ ={b0, state_map, psk_map, bad, dec_map}(Red_ROM.WAKE_O, Game5)
   /\ (forall a b ca, (forall cb caf, (msg3_data a b ca cb, caf) \notin Game5.prfkey_map{2})
-        => (msg1_data a b, ca) \notin RO.m{1})
+        => (msg1_data a b, ca) \notin NROc.RO.m{1})
   /\ (forall a b ca cb, (forall caf, (msg3_data a b ca cb, caf) \notin Game5.prfkey_map{2})
-        => (msg2_data a b ca, cb) \notin RO.m{1})
+        => (msg2_data a b ca, cb) \notin NROc.RO.m{1})
   /\ (forall a b ca cb caf, (msg3_data a b ca cb, caf) \in Game5.prfkey_map{2} =>
          exists na nb, Game5.prfkey_map{2}.[(msg3_data a b ca cb, caf)] = Some (na, nb) /\
-                       RO.m{1}.[(msg1_data a b, ca)] = Some na /\
-                       RO.m{1}.[(msg2_data a b ca, cb)] = Some nb)
+                       NROc.RO.m{1}.[(msg1_data a b, ca)] = Some na /\
+                       NROc.RO.m{1}.[(msg2_data a b ca, cb)] = Some nb)
   ) _ Game5_inv_send_msg3 => //.
   proc; inline*.
   sp; wp; if=> //.
@@ -2461,15 +1688,15 @@ wp; call (:
   smt(get_setE).
 
 - conseq (: ={res}
-  /\ ={b0, state_map, psk_map, bad, dec_map}(Red_ROM_ideal.WAKE_O, Game5)
+  /\ ={b0, state_map, psk_map, bad, dec_map}(Red_ROM.WAKE_O, Game5)
   /\ (forall a b ca, (forall cb caf, (msg3_data a b ca cb, caf) \notin Game5.prfkey_map{2})
-        => (msg1_data a b, ca) \notin RO.m{1})
+        => (msg1_data a b, ca) \notin NROc.RO.m{1})
   /\ (forall a b ca cb, (forall caf, (msg3_data a b ca cb, caf) \notin Game5.prfkey_map{2})
-        => (msg2_data a b ca, cb) \notin RO.m{1})
+        => (msg2_data a b ca, cb) \notin NROc.RO.m{1})
   /\ (forall a b ca cb caf, (msg3_data a b ca cb, caf) \in Game5.prfkey_map{2} =>
          exists na nb, Game5.prfkey_map{2}.[(msg3_data a b ca cb, caf)] = Some (na, nb) /\
-                       RO.m{1}.[(msg1_data a b, ca)] = Some na /\
-                       RO.m{1}.[(msg2_data a b ca, cb)] = Some nb)
+                       NROc.RO.m{1}.[(msg1_data a b, ca)] = Some na /\
+                       NROc.RO.m{1}.[(msg2_data a b ca, cb)] = Some nb)
   ) _ Game5_inv_send_fin => //.
 - proc; inline*.
   sp; wp ^if ^if; if=> //.
@@ -2495,266 +1722,28 @@ wp; call (:
   smt().
 
 - conseq (: ={res}
-  /\ ={b0, state_map, psk_map, bad, dec_map}(Red_ROM_ideal.WAKE_O, Game5)
+  /\ ={b0, state_map, psk_map, bad, dec_map}(Red_ROM.WAKE_O, Game5)
   /\ (forall a b ca, (forall cb caf, (msg3_data a b ca cb, caf) \notin Game5.prfkey_map{2})
-        => (msg1_data a b, ca) \notin RO.m{1})
+        => (msg1_data a b, ca) \notin NROc.RO.m{1})
   /\ (forall a b ca cb, (forall caf, (msg3_data a b ca cb, caf) \notin Game5.prfkey_map{2})
-        => (msg2_data a b ca, cb) \notin RO.m{1})
+        => (msg2_data a b ca, cb) \notin NROc.RO.m{1})
   /\ (forall a b ca cb caf, (msg3_data a b ca cb, caf) \in Game5.prfkey_map{2} =>
          exists na nb, Game5.prfkey_map{2}.[(msg3_data a b ca cb, caf)] = Some (na, nb) /\
-                       RO.m{1}.[(msg1_data a b, ca)] = Some na /\
-                       RO.m{1}.[(msg2_data a b ca, cb)] = Some nb)
+                       NROc.RO.m{1}.[(msg1_data a b, ca)] = Some na /\
+                       NROc.RO.m{1}.[(msg2_data a b ca, cb)] = Some nb)
   ) _ Game5_inv_rev_skey => //.
   by sim />.
 
 - conseq (: ={res}
-  /\ ={b0, state_map, psk_map, bad, dec_map}(Red_ROM_ideal.WAKE_O, Game5)
+  /\ ={b0, state_map, psk_map, bad, dec_map}(Red_ROM.WAKE_O, Game5)
   /\ (forall a b ca, (forall cb caf, (msg3_data a b ca cb, caf) \notin Game5.prfkey_map{2})
-        => (msg1_data a b, ca) \notin RO.m{1})
+        => (msg1_data a b, ca) \notin NROc.RO.m{1})
   /\ (forall a b ca cb, (forall caf, (msg3_data a b ca cb, caf) \notin Game5.prfkey_map{2})
-        => (msg2_data a b ca, cb) \notin RO.m{1})
+        => (msg2_data a b ca, cb) \notin NROc.RO.m{1})
   /\ (forall a b ca cb caf, (msg3_data a b ca cb, caf) \in Game5.prfkey_map{2} =>
          exists na nb, Game5.prfkey_map{2}.[(msg3_data a b ca cb, caf)] = Some (na, nb) /\
-                       RO.m{1}.[(msg1_data a b, ca)] = Some na /\
-                       RO.m{1}.[(msg2_data a b ca, cb)] = Some nb)
-  ) _ Game5_inv_test => //.
-  by sim />.
-
-auto => />.
-smt(Game5_undef emptyE).
-
-
-(* Proof for the real side *)
-transitivity* {1} { r <@ MainD(Red_ROM_real(A), RO).distinguish(); }.
-
-+ inline*.
-  wp.
-  call (: ={b0, state_map, psk_map, bad}(Game4, Red_ROM_real.WAKE_O)
-       /\ (forall h, h \in Game4.dec_map{1} <=> h \in Red_ROM_real.WAKE_O.dec_map{2})
-       /\ (forall c ad n, (exists pk, Game4.dec_map{1}.[(pk, ad, c)] = Some n) <=> RO.m{2}.[(ad, c)] = Some n)
-       /\ (forall a b ca cb, ((a, b), msg2_data a b ca, cb) \in Game4.dec_map => ((a, b), msg1_data a b, ca) \in Game4.dec_map){1}
-       /\ (forall a b ca cb caf, ((a, b), msg3_data a b ca cb, caf) \in Game4.dec_map => ((a, b), msg2_data a b ca, cb) \in Game4.dec_map){1}
-  ) => //.
-
-  - by proc; sp; if; auto.
-
-  - proc; inline*.
-    sp; wp; if=> //.
-    seq 1 1 : (#pre /\ ={ca}); 1: by auto.
-    sp; if=> //.
-    + smt().
-    + rcondt {2} ^if; 1: by auto=> /#. 
-      auto=> />.
-      smt(get_setE).
-    by auto=> /#.
-  
-   - proc; inline*.
-     sp; wp; if=> //. 
-     match; 1,2: smt().
-     + by auto=> />.
-     move=> nal nar.
-     seq 1 1 : (#pre /\ ={cb}); 1: by auto.
-     sp; if=> //.
-     + smt().
-     + rcondt {2} ^if; 1: by auto=> /#. 
-       auto=> />.
-       smt(get_setE).
-     by auto=> /#.
-
-   - proc; inline*.
-     sp; wp; if=> //. 
-     sp; match = => //.
-     + smt().
-     move=> s m1.
-     sp; match; 1: smt().
-     + move => /> *; smt().
-     + by auto=> />.
-     move=> nbl nbr.
-     seq 1 1 : (#pre /\ ={caf}); 1: by auto.
-     sp; if=> //.
-     + smt().
-     + rcondt {2} ^if; 1: by auto=> /#.
-       rcondf {2} ^if.
-       + auto=> />.
-         smt(mem_set).
-       rcondf {2} ^if.
-       + auto=> />.
-         smt(mem_set).
-       swap {2} ^r1<$ @ ^ok<-.
-       seq 1 1 : (#pre /\ ok{1} = r1{2}); 1: by auto => />.
-       auto=> />.
-       smt(get_setE).
-    by auto=> /#.
-  
-   - proc; inline*.
-     sp; wp ^if ^if; if=> //. 
-     sp; match = => //.
-     + smt().
-     move=> s m1 m2.
-     sp; match; 1,2: smt().
-     + by auto=> />.
-     move=> nokl nokr.
-     rcondf {2} ^if; 1: by auto=> /#.
-     rcondf {2} ^if; 1: by auto=> /#.
-     auto=> />.
-     smt(get_setE).
-  
-   - by sim />.
-   
-   - by sim />.
-
-   auto=> />.
-   smt(emptyE).
-  
-rewrite equiv [{1} 1 (FullEager.RO_LRO (Red_ROM_real(A)) _)]; 1: by move=> _; exact dnonce_ll.
-inline*.
-wp; call (: 
-  ={b0, state_map, psk_map, bad, dec_map}(Red_ROM_real.WAKE_O, Game5)
-  /\ (forall a b ca, (forall cb caf, (msg3_data a b ca cb, caf) \notin Game5.prfkey_map{2})
-        => (msg1_data a b, ca) \notin RO.m{1})
-  /\ (forall a b ca cb, (forall caf, (msg3_data a b ca cb, caf) \notin Game5.prfkey_map{2})
-        => (msg2_data a b ca, cb) \notin RO.m{1})
-  /\ (forall a b ca cb caf, (msg3_data a b ca cb, caf) \in Game5.prfkey_map{2} =>
-         exists na nb, Game5.prfkey_map{2}.[(msg3_data a b ca cb, caf)] = Some (na, nb) /\
-                       RO.m{1}.[(msg1_data a b, ca)] = Some na /\
-                       RO.m{1}.[(msg2_data a b ca, cb)] = Some nb)
-  /\ (Game5_inv_full Game5.state_map Game5.dec_map Game5.prfkey_map){2}
-) => //.
-
-- by sim />.
-
-- conseq (: ={res}
-  /\ ={b0, state_map, psk_map, bad, dec_map}(Red_ROM_real.WAKE_O, Game5)
-  /\ (forall a b ca, (forall cb caf, (msg3_data a b ca cb, caf) \notin Game5.prfkey_map{2})
-        => (msg1_data a b, ca) \notin RO.m{1})
-  /\ (forall a b ca cb, (forall caf, (msg3_data a b ca cb, caf) \notin Game5.prfkey_map{2})
-        => (msg2_data a b ca, cb) \notin RO.m{1})
-  /\ (forall a b ca cb caf, (msg3_data a b ca cb, caf) \in Game5.prfkey_map{2} =>
-         exists na nb, Game5.prfkey_map{2}.[(msg3_data a b ca cb, caf)] = Some (na, nb) /\
-                       RO.m{1}.[(msg1_data a b, ca)] = Some na /\
-                       RO.m{1}.[(msg2_data a b ca, cb)] = Some nb)
-  ) _ Game5_inv_send_msg1 => //.
-  proc; inline*.
-  sp; wp; if=> //.
-  by auto=> />.
-
-- conseq (: ={res}
-  /\ ={b0, state_map, psk_map, bad, dec_map}(Red_ROM_real.WAKE_O, Game5)
-  /\ (forall a b ca, (forall cb caf, (msg3_data a b ca cb, caf) \notin Game5.prfkey_map{2})
-        => (msg1_data a b, ca) \notin RO.m{1})
-  /\ (forall a b ca cb, (forall caf, (msg3_data a b ca cb, caf) \notin Game5.prfkey_map{2})
-        => (msg2_data a b ca, cb) \notin RO.m{1})
-  /\ (forall a b ca cb caf, (msg3_data a b ca cb, caf) \in Game5.prfkey_map{2} =>
-         exists na nb, Game5.prfkey_map{2}.[(msg3_data a b ca cb, caf)] = Some (na, nb) /\
-                       RO.m{1}.[(msg1_data a b, ca)] = Some na /\
-                       RO.m{1}.[(msg2_data a b ca, cb)] = Some nb)
-  ) _ Game5_inv_send_msg2 => //.
-  proc; inline*.
-  sp; wp; if=> //.
-  by sp; match =; auto=> />.
-
-- conseq (: ={res}
-  /\ ={b0, state_map, psk_map, bad, dec_map}(Red_ROM_real.WAKE_O, Game5)
-  /\ (forall a b ca, (forall cb caf, (msg3_data a b ca cb, caf) \notin Game5.prfkey_map{2})
-        => (msg1_data a b, ca) \notin RO.m{1})
-  /\ (forall a b ca cb, (forall caf, (msg3_data a b ca cb, caf) \notin Game5.prfkey_map{2})
-        => (msg2_data a b ca, cb) \notin RO.m{1})
-  /\ (forall a b ca cb caf, (msg3_data a b ca cb, caf) \in Game5.prfkey_map{2} =>
-         exists na nb, Game5.prfkey_map{2}.[(msg3_data a b ca cb, caf)] = Some (na, nb) /\
-                       RO.m{1}.[(msg1_data a b, ca)] = Some na /\
-                       RO.m{1}.[(msg2_data a b ca, cb)] = Some nb)
-  ) _ Game5_inv_send_msg3 => //.
-  proc; inline*.
-  sp; wp; if=> //.
-  sp; match = => //.
-  + smt().
-  move=> s m1.
-  sp; match = => //.
-  + by auto.
-  move=> nb.
-  seq 1 1 : (#pre /\ ={caf}); 1: by auto.
-  sp; if=> //.
-  rcondt {1} ^if.
-  + auto=> />.
-    move=> &hr _ dm _ sm _ inv1 inv2 inv3 invr1 invr2 invr3 invr4 invr5 /domE/some_oget sms /negb_or [_ cafnin] r _. 
-    rewrite -sm in sms.
-    case: (invr5 a{m0} i{m0}); rewrite sms //=.
-    move=> /> 4!->> _.
-    exact inv1.
-  rcondt {1} ^if.
-  + auto=> />.
-    move=> &hr _ dm _ sm _ inv1 inv2 inv3 invr1 invr2 invr3 invr4 invr5 /domE/some_oget sms /negb_or [_ cafnin] r _ r1 _. 
-    rewrite -sm in sms.
-    case: (invr5 a{m0} i{m0}) ; rewrite sms //=.
-    move=> /> 4!->> _.
-    rewrite mem_set /#.
-  outline {2} 3 by {(na, nb') <@ S.sample(dnonce, dnonce);}. 
-  wp; rewrite equiv [{2} 3 sample_sample2].
-  inline*.
-  auto=> />.
-  move=> &1 &2 _ dm _ sm _ inv1 inv2 inv3 invr1 invr2 invr3 invr4 invr5 /domE/some_oget sms /negb_or [_ cafnin] r _ r1 _. 
-  rewrite get_set_sameE //=.
-  rewrite -sm in sms.
-  case: (invr5 a{2} i{2}); rewrite sms //=.
-  smt(get_setE).
-
-- conseq (: ={res}
-  /\ ={b0, state_map, psk_map, bad, dec_map}(Red_ROM_real.WAKE_O, Game5)
-  /\ (forall a b ca, (forall cb caf, (msg3_data a b ca cb, caf) \notin Game5.prfkey_map{2})
-        => (msg1_data a b, ca) \notin RO.m{1})
-  /\ (forall a b ca cb, (forall caf, (msg3_data a b ca cb, caf) \notin Game5.prfkey_map{2})
-        => (msg2_data a b ca, cb) \notin RO.m{1})
-  /\ (forall a b ca cb caf, (msg3_data a b ca cb, caf) \in Game5.prfkey_map{2} =>
-         exists na nb, Game5.prfkey_map{2}.[(msg3_data a b ca cb, caf)] = Some (na, nb) /\
-                       RO.m{1}.[(msg1_data a b, ca)] = Some na /\
-                       RO.m{1}.[(msg2_data a b ca, cb)] = Some nb)
-  ) _ Game5_inv_send_fin => //.
-- proc; inline*.
-  sp; wp ^if ^if; if=> //.
-  sp; match = => //.
-  + smt().
-  move=> s m1 m2.
-  sp; match = => //.
-  + by auto.
-  move=> nok.
-  rcondf {1} ^if.
-  + auto=> />.
-    move=> &hr dm _ sm _ inv1 inv2 inv3 invr1 invr2 invr3 invr4 invr5 /domE/some_oget sms r _.
-    rewrite -sm in sms.
-    case: (invr5 b{m0} j{m0}) ; rewrite sms //=.
-    smt().
-  rcondf {1} ^if.
-  + auto=> />.
-    move=> &hr dm _ sm _ inv1 inv2 inv3 invr1 invr2 invr3 invr4 invr5 /domE/some_oget sms r _ r2 _.
-    rewrite -sm in sms.
-    case: (invr5 b{m0} j{m0}) ; rewrite sms //=.
-    smt().
-  auto=> />.
-  smt().
-
-- conseq (: ={res}
-  /\ ={b0, state_map, psk_map, bad, dec_map}(Red_ROM_real.WAKE_O, Game5)
-  /\ (forall a b ca, (forall cb caf, (msg3_data a b ca cb, caf) \notin Game5.prfkey_map{2})
-        => (msg1_data a b, ca) \notin RO.m{1})
-  /\ (forall a b ca cb, (forall caf, (msg3_data a b ca cb, caf) \notin Game5.prfkey_map{2})
-        => (msg2_data a b ca, cb) \notin RO.m{1})
-  /\ (forall a b ca cb caf, (msg3_data a b ca cb, caf) \in Game5.prfkey_map{2} =>
-         exists na nb, Game5.prfkey_map{2}.[(msg3_data a b ca cb, caf)] = Some (na, nb) /\
-                       RO.m{1}.[(msg1_data a b, ca)] = Some na /\
-                       RO.m{1}.[(msg2_data a b ca, cb)] = Some nb)
-  ) _ Game5_inv_rev_skey => //.
-  by sim />.
-
-- conseq (: ={res}
-  /\ ={b0, state_map, psk_map, bad, dec_map}(Red_ROM_real.WAKE_O, Game5)
-  /\ (forall a b ca, (forall cb caf, (msg3_data a b ca cb, caf) \notin Game5.prfkey_map{2})
-        => (msg1_data a b, ca) \notin RO.m{1})
-  /\ (forall a b ca cb, (forall caf, (msg3_data a b ca cb, caf) \notin Game5.prfkey_map{2})
-        => (msg2_data a b ca, cb) \notin RO.m{1})
-  /\ (forall a b ca cb caf, (msg3_data a b ca cb, caf) \in Game5.prfkey_map{2} =>
-         exists na nb, Game5.prfkey_map{2}.[(msg3_data a b ca cb, caf)] = Some (na, nb) /\
-                       RO.m{1}.[(msg1_data a b, ca)] = Some na /\
-                       RO.m{1}.[(msg2_data a b ca, cb)] = Some nb)
+                       NROc.RO.m{1}.[(msg1_data a b, ca)] = Some na /\
+                       NROc.RO.m{1}.[(msg2_data a b ca, cb)] = Some nb)
   ) _ Game5_inv_test => //.
   by sim />.
 
@@ -2766,17 +1755,17 @@ qed.
 (* ------------------------------------------------------------------------------------------ *)
 (* Step 5: Apply the PRF assumption. *)
 
-lemma Step5_real &m:
-    `|Pr[E_GWAKE(Game5, A).run(false) @ &m : res] - Pr[E_GWAKE(Game6, A).run(false) @ &m : res]|
+lemma Step5 bit &m:
+    `|Pr[E_GWAKE(Game5, A).run(bit) @ &m : res] - Pr[E_GWAKE(Game6, A).run(bit) @ &m : res]|
   = 
-    `|Pr[E_GPRF(PRF0, Red_PRF_real(A)).run() @ &m : res] - Pr[E_GPRF(PRF1, Red_PRF_real(A)).run() @ &m : res]|.
+    `|Pr[E_GPRF(PRF0, Red_PRF(A)).run(bit) @ &m : res] - Pr[E_GPRF(PRF1, Red_PRF(A)).run(bit) @ &m : res]|.
 proof.
 do! congr.
 + byequiv => //.
   proc; inline*.
   wp.
   call (:
-        ={b0, psk_map, state_map, dec_map, bad}(Game5, Red_PRF_real.WAKE_O)
+        ={b0, psk_map, state_map, dec_map, bad}(Game5, Red_PRF.WAKE_O)
      /\ ={prfkey_map}(Game5, PRFb)
      /\ (Game5_inv_full Game5.state_map Game5.dec_map Game5.prfkey_map){1}
   )=> //.
@@ -2784,19 +1773,20 @@ do! congr.
   - by sim />.
 
   - conseq (: ={res}
-     /\ ={psk_map, state_map, dec_map, bad}(Game5, Red_PRF_real.WAKE_O)
+     /\ ={psk_map, state_map, dec_map, bad}(Game5, Red_PRF.WAKE_O)
      /\ ={prfkey_map}(Game5, PRFb)
     ) Game5_inv_send_msg1 _ => //.
-    by sim />.
+   proc.    
+by sim />.
 
   - conseq (: ={res}
-     /\ ={psk_map, state_map, dec_map, bad}(Game5, Red_PRF_real.WAKE_O)
+     /\ ={psk_map, state_map, dec_map, bad}(Game5, Red_PRF.WAKE_O)
      /\ ={prfkey_map}(Game5, PRFb)
     ) Game5_inv_send_msg2 _ => //.
     by sim />.
 
   - conseq (: ={res}
-     /\ ={psk_map, state_map, dec_map, bad}(Game5, Red_PRF_real.WAKE_O)
+     /\ ={psk_map, state_map, dec_map, bad}(Game5, Red_PRF.WAKE_O)
      /\ ={prfkey_map}(Game5, PRFb)
     ) Game5_inv_send_msg3 _ => //.
     proc; inline*.
@@ -2819,7 +1809,7 @@ do! congr.
     smt(get_setE).
 
   - conseq (: ={res}
-     /\ ={psk_map, state_map, dec_map, bad}(Game5, Red_PRF_real.WAKE_O)
+     /\ ={psk_map, state_map, dec_map, bad}(Game5, Red_PRF.WAKE_O)
      /\ ={prfkey_map}(Game5, PRFb)
     ) Game5_inv_send_fin _ => //.
      proc; inline*.
@@ -2838,13 +1828,13 @@ do! congr.
      smt(get_setE).
 
   - conseq (: ={res}
-     /\ ={psk_map, state_map, dec_map, bad}(Game5, Red_PRF_real.WAKE_O)
+     /\ ={psk_map, state_map, dec_map, bad}(Game5, Red_PRF.WAKE_O)
      /\ ={prfkey_map}(Game5, PRFb)
     ) Game5_inv_rev_skey _ => //.
     by sim />.
 
   - conseq (: ={res}
-     /\ ={psk_map, state_map, dec_map, bad}(Game5, Red_PRF_real.WAKE_O)
+     /\ ={psk_map, state_map, dec_map, bad}(Game5, Red_PRF.WAKE_O)
      /\ ={prfkey_map}(Game5, PRFb)
     ) Game5_inv_test _ => //.
     by sim />.
@@ -2856,168 +1846,7 @@ byequiv => //.
 proc; inline *.
 wp.
 call (:
-      ={b0, psk_map, state_map, dec_map, bad}(Game6, Red_PRF_real.WAKE_O)
-   /\ ={prfkey_map}(Game6, PRFb)
-   /\ (forall a b m1 m2 m3, ((a, b), msg3_data a b m1 m2, m3) \in Game6.dec_map{1} <=> ((msg3_data a b m1 m2, m3), (a, b)) \in PRF1.cache{2})
-   /\ (forall a b m1 m2 m3 k, PRF1.cache.[((msg3_data a b m1 m2, m3), (a, b))]{2} = Some k => Game6.sk_map.[((a, m1), m2, m3)]{1} = Some k)
-   /\ (forall a b m1 m2 m3, ((a, b), msg3_data a b m1 m2, m3) \in Game6.dec_map <=> (msg3_data a b m1 m2, m3) \in Game6.prfkey_map){1}
-)=> //. 
-
-- by sim />.
-
-- proc; inline*. 
-  sp; wp; if => //.
-  auto => />.
-  smt(get_setE).
-
-- proc; inline*.
-  sp; wp; if => //.
-  match = => //.
-  + by auto => />. 
-  auto => />.
-  smt(get_setE).
-
-- proc; inline*.
-  sp; wp; if=> //. 
-  sp; match = => //.
-  + smt().
-  move=> s m1.
-  sp; match =.
-  + smt().
-  + by auto=> />.
-  move=> nb.
-  seq 1 1 : (#pre /\ ={caf}); 1: by auto.
-  sp; if=> //.
-  rcondt{2} ^if.
-  + auto=> />.
-    smt().
-  match Some {2} ^match.
-  + auto=> />.
-    smt(get_setE). 
-  rcondt{2} ^if.
-  + auto => />.
-    smt().
-  auto=> />.
-  smt(get_setE).
-
-- proc; inline*.
-  sp; wp ^if ^if; if=> //. 
-  sp; match = => //.
-  + smt().
-  move=> s m1 m2.
-  sp; match =.
-  + smt().
-  + by auto=> />.
-  move=> nok.
-  match Some {2} ^match.
-  + auto=> />.
-    smt().
-  rcondf{2} ^if.
-  + auto => />.
-    smt().
-  auto=> />.
-  smt().
-
-- by sim />.
-
-- by sim />.
-
-auto => />.
-smt(emptyE).
-qed.
-
-
-lemma Step5_ideal &m:
-    `|Pr[E_GWAKE(Game5, A).run(true) @ &m : res] - Pr[E_GWAKE(Game6, A).run(true) @ &m : res]|
-  = 
-    `|Pr[E_GPRF(PRF0, Red_PRF_ideal(A)).run() @ &m : res] - Pr[E_GPRF(PRF1, Red_PRF_ideal(A)).run() @ &m : res]|.
-proof.
-do! congr.
-+ byequiv => //.
-  proc; inline*.
-  wp.
-  call (:
-        ={b0, psk_map, state_map, dec_map, bad}(Game5, Red_PRF_ideal.WAKE_O)
-     /\ ={prfkey_map}(Game5, PRFb)
-     /\ (Game5_inv_full Game5.state_map Game5.dec_map Game5.prfkey_map){1}
-  )=> //.
-
-  - by sim />.
-
-  - conseq (: ={res}
-     /\ ={psk_map, state_map, dec_map, bad}(Game5, Red_PRF_ideal.WAKE_O)
-     /\ ={prfkey_map}(Game5, PRFb)
-    ) Game5_inv_send_msg1 _ => //.
-    by sim />.
-
-  - conseq (: ={res}
-     /\ ={psk_map, state_map, dec_map, bad}(Game5, Red_PRF_ideal.WAKE_O)
-     /\ ={prfkey_map}(Game5, PRFb)
-    ) Game5_inv_send_msg2 _ => //.
-    by sim />.
-
-  - conseq (: ={res}
-     /\ ={psk_map, state_map, dec_map, bad}(Game5, Red_PRF_ideal.WAKE_O)
-     /\ ={prfkey_map}(Game5, PRFb)
-    ) Game5_inv_send_msg3 _ => //.
-    proc; inline*.
-    sp; wp; if=> //. 
-    sp; match = => //.
-    + smt().
-    move=> s m1.
-    sp; match =.
-    + smt().
-    + by auto=> />.
-    move=> nb.
-    seq 1 1 : (#pre /\ ={caf}); 1: by auto.
-    sp; if=> //.
-    rcondt{2} ^if.
-    + auto=> />. 
-      smt().
-    match Some {2} ^match.
-    + by auto => />; smt(mem_set get_setE).
-    auto => />. 
-    smt(get_setE).
-
-  - conseq (: ={res}
-     /\ ={psk_map, state_map, dec_map, bad}(Game5, Red_PRF_ideal.WAKE_O)
-     /\ ={prfkey_map}(Game5, PRFb)
-    ) Game5_inv_send_fin _ => //.
-     proc; inline*.
-     sp; wp ^if ^if; if=> //. 
-     sp; match = => //.
-     + smt().
-     move=> s m1 m2.
-     sp; match =.
-     + smt().
-     + by auto=> />.
-     move=> nok.
-     match Some {2} ^match.
-     + auto=> />.
-       smt().
-     auto => />.
-     smt(get_setE).
-
-  - conseq (: ={res}
-     /\ ={psk_map, state_map, dec_map, bad}(Game5, Red_PRF_ideal.WAKE_O)
-     /\ ={prfkey_map}(Game5, PRFb)
-    ) Game5_inv_rev_skey _ => //.
-    by sim />.
-
-  - conseq (: ={res}
-     /\ ={psk_map, state_map, dec_map, bad}(Game5, Red_PRF_ideal.WAKE_O)
-     /\ ={prfkey_map}(Game5, PRFb)
-    ) Game5_inv_test _ => //.
-    by sim />.
-
-  auto => />.
-  smt(emptyE Game5_undef).
-
-byequiv => //.
-proc; inline *.
-wp.
-call (:
-      ={b0, psk_map, state_map, dec_map, bad}(Game6, Red_PRF_ideal.WAKE_O)
+      ={b0, psk_map, state_map, dec_map, bad}(Game6, Red_PRF.WAKE_O)
    /\ ={prfkey_map}(Game6, PRFb)
    /\ (forall a b m1 m2 m3, ((a, b), msg3_data a b m1 m2, m3) \in Game6.dec_map{1} <=> ((msg3_data a b m1 m2, m3), (a, b)) \in PRF1.cache{2})
    /\ (forall a b m1 m2 m3 k, PRF1.cache.[((msg3_data a b m1 m2, m3), (a, b))]{2} = Some k => Game6.sk_map.[((a, m1), m2, m3)]{1} = Some k)
@@ -3238,11 +2067,11 @@ auto=> />.
 by smt(emptyE).
 qed.
 
-
-
 lemma final &m: `| Pr[E_GWAKE(GWAKEb(NSL), A).run(false) @ &m : res] - Pr[E_GWAKE(GWAKEb(NSL), A).run(true) @ &m : res]|
-  <=  `|Pr[E_GAEAD(GAEAD0, Red_AEAD_ideal(A)).run() @ &m : res] - Pr[E_GAEAD(GAEAD1, Red_AEAD_ideal(A)).run() @ &m : res]|
-      + `|Pr[E_GPRF(PRF0, Red_PRF_ideal(A)).run() @ &m : res] - Pr[E_GPRF(PRF1, Red_PRF_ideal(A)).run() @ &m : res]|
+  <= `|Pr[E_GAEAD(GAEAD0, Red_AEAD(A)).run(false) @ &m : res] - Pr[E_GAEAD(GAEAD1, Red_AEAD(A)).run(false) @ &m : res]|
+      + `|Pr[E_GAEAD(GAEAD0, Red_AEAD(A)).run(true) @ &m : res] - Pr[E_GAEAD(GAEAD1, Red_AEAD(A)).run(true) @ &m : res]|
+      + `|Pr[E_GPRF(PRF0, Red_PRF(A)).run(false) @ &m : res] - Pr[E_GPRF(PRF1, Red_PRF(A)).run(false) @ &m : res]|
+      + `|Pr[E_GPRF(PRF0, Red_PRF(A)).run(true) @ &m : res] - Pr[E_GPRF(PRF1, Red_PRF(A)).run(true) @ &m : res]|
       + 2%r * ((q_m1 + q_m2 + q_m3) ^ 2)%r * mu1 dctxt (mode dctxt).
 proof.
 rewrite !Step0.
